added uint32s and uint32 arrays to GenericMarshalling

lib/Marshalling/GenericMarshalling.i.dfy
@@ -40,24 +40,28 @@ export extends S
 type Key = KeyType.Key
 type Message = ValueMessage.Message
 
-datatype G = GUint64
+datatype G = GUint32
+           | GUint64
            | GArray(elt:G)
            | GTuple(t:seq<G>)
            | GByteArray
            | GMessage
+           | GUint32Array
            | GUint64Array
            | GKeyArray
            | GMessageArray
            | GTaggedUnion(cases:seq<G>)
            | GPackedKV
 
-datatype V = VUint64(u:uint64)
+datatype V = VUint32(v:uint32)
+           | VUint64(u:uint64)
            | VArray(a:seq<V>)
            | VTuple(t:seq<V>)
            | VByteArray(b:seq<byte>)
            | VMessage(m:Message)
            | VKeyArray(ka:seq<Key>)
            | VMessageArray(ma:seq<Message>)
+           | VUint32Array(va:seq<uint32>)
            | VUint64Array(ua:seq<uint64>)
            | VCase(c:uint64, val:V)
            | VPackedKV(pkv: Pkv)
@@ -65,6 +69,7 @@ datatype V = VUint64(u:uint64)
 predicate ValInGrammar(val:V, grammar:G)
 {
     match val
+        case VUint32(_) => grammar.GUint32?
         case VUint64(_) => grammar.GUint64?
         case VArray(a)  => grammar.GArray? && forall v :: v in a ==> ValInGrammar(v, grammar.elt)
         case VTuple(t)  => grammar.GTuple? && |t| == |grammar.t|
@@ -73,6 +78,7 @@ predicate ValInGrammar(val:V, grammar:G)
         case VMessage(b) => grammar.GMessage?
         case VKeyArray(b) => grammar.GKeyArray?
         case VMessageArray(b) => grammar.GMessageArray?
+        case VUint32Array(va) => grammar.GUint32Array?
         case VUint64Array(ua) => grammar.GUint64Array?
         case VCase(c, v) => grammar.GTaggedUnion? && (c as int) < |grammar.cases| && ValInGrammar(v, grammar.cases[c])
         case VPackedKV(pkv) => grammar.GPackedKV?
@@ -82,6 +88,7 @@ predicate ValInGrammar(val:V, grammar:G)
 predicate ValidGrammar(grammar:G) 
 {
     match grammar
+        case GUint32 => true
         case GUint64 => true
         case GArray(elt) => ValidGrammar(elt)
         case GTuple(t) => |t| < 0x1_0000_0000_0000_0000 && (forall g :: g in t ==> ValidGrammar(g))
@@ -89,6 +96,7 @@ predicate ValidGrammar(grammar:G)
         case GMessage => true
         case GKeyArray => true
         case GMessageArray => true
+        case GUint32Array => true
         case GUint64Array => true
         case GTaggedUnion(cases) => |cases| < 0x1_0000_0000_0000_0000 && (forall g :: g in cases ==> ValidGrammar(g))
         case GPackedKV => true
@@ -103,6 +111,7 @@ predicate ValidMessage(m: Message)
 predicate ValidVal(val:V)
 {
     match val
+        case VUint32(_)    => true
         case VUint64(_)    => true
         case VArray(a)     => |a| < 0x1_0000_0000_0000_0000 && forall v :: v in a ==> ValidVal(v)
         case VTuple(t)     => |t| < 0x1_0000_0000_0000_0000 && forall v :: v in t ==> ValidVal(v)
@@ -110,6 +119,7 @@ predicate ValidVal(val:V)
         case VKeyArray(ka) => |ka| < 0x1_0000_0000_0000_0000
         case VMessage(m) => ValidMessage(m)
         case VMessageArray(ma) => |ma| < 0x1_0000_0000_0000_0000 && forall v :: v in ma ==> ValidMessage(v)
+        case VUint32Array(va) => |va| < 0x1_0000_0000
         case VUint64Array(ua) => |ua| < 0x1_0000_0000_0000_0000
         case VCase(c, v) => ValidVal(v)
         case VPackedKV(pkv) => PackedKV.WF(pkv)
@@ -127,6 +137,7 @@ function SizeOfV(val:V) : int
     ensures SizeOfV(val) >= 0;
 {
     match val
+        case VUint32(_)     => 4
         case VUint64(_)     => 8
         case VArray(a)      => 8 + SeqSum(a)     // 8 bytes for length
         case VTuple(t)      => SeqSum(t)
@@ -134,18 +145,50 @@ function SizeOfV(val:V) : int
         case VKeyArray(ka)  => 4 + WeightKeySeq(ka)
         case VMessage(m)  => 4 + WeightMessage(m)
         case VMessageArray(ma)  => 4 + WeightMessageSeq(ma)
+        case VUint32Array(b)  => 4 + 4*|b|          // 4 bytes for a length field
         case VUint64Array(b)  => 8 + 8*|b|          // 8 bytes for a length field
         case VCase(c, v)  => 8 + SizeOfV(v)     // 8 bytes for the case identifier
         case VPackedKV(pkv)  => PackedKV.SizeOfPkv(pkv)
 }
 
-function parse_Uint64(data:seq<byte>) : (Option<V>, seq<byte>)
+function parse_Uint32(data:seq<byte>) : (Option<V>, seq<byte>)
     requires |data| < 0x1_0000_0000_0000_0000;
+{
+    if (|data| as uint64) >= Uint32Size() then
+        (Some(VUint32(unpack_LittleEndian_Uint32(data[..Uint32Size()]))), data[Uint32Size()..])
+    else
+        (None, [])
+}
+
+function parse_Uint64(data:seq<byte>) : (result: (Option<V>, seq<byte>))
+  requires |data| < 0x1_0000_0000_0000_0000;
+  ensures result.0.Some? ==> result.0.value.VUint64?
 {
     if (|data| as uint64) >= Uint64Size() then
         (Some(VUint64(unpack_LittleEndian_Uint64(data[..Uint64Size()]))), data[Uint64Size()..])
     else
         (None, [])
+}
+
+method ParseUint32(data:seq<byte>, index:uint64) returns (success:bool, v:V, rest_index:uint64)
+    requires (index as int) <= |data|
+    requires |data| < 0x1_0000_0000_0000_0000;
+    ensures  (rest_index as int) <= |data|
+    ensures  var (v', rest') := parse_Uint32(data[index..]);
+             var v_opt := if success then Some(v) else None();
+             v_opt == v' && data[rest_index..] == rest';
+{
+    if |data| as uint64 - index >= 4 {
+        var result := Unpack_LittleEndian_Uint32(data, index);
+        success := true;
+        v := VUint32(result);
+        rest_index := index + Uint32Size();
+
+        assert data[index..][..Uint32Size()] == data[index .. index + Uint32Size()];
+    } else {
+        success := false;
+        rest_index := (|data| as uint64);
+    }
 }
 
 method ParseUint64(data:seq<byte>, index:uint64) returns (success:bool, v:V, rest_index:uint64)
@@ -340,7 +383,9 @@ function parse_Array(data:seq<byte>, eltType:G) : (Option<V>, seq<byte>)
 {
     var (len, rest) := parse_Uint64(data);
     if !len.None? then
-        var (contents, remainder) := parse_Array_contents(rest, eltType, len.value.u);
+        assert len.value.VUint64?;
+        var len64: uint64 := len.value.u;
+        var (contents, remainder) := parse_Array_contents(rest, eltType, len64);
         if !contents.None? then
             (Some(VArray(contents.value)), remainder)
         else
@@ -660,6 +705,50 @@ method ParseByteArray(data:seq<byte>, index:uint64) returns (success:bool, v:seq
     }
 }
 
+function parse_Uint32Array(data:seq<byte>) : (Option<V>, seq<byte>)
+    requires |data| < 0x1_0000_0000_0000_0000;
+{
+  if |data| >= 4 then (
+    var len := unpack_LittleEndian_Uint32(data[..4]) as uint64;
+    if len <= (|data| as uint64 - 4) / 4 then
+        (Some(VUint32Array(unpack_LittleEndian_Uint32_Seq(data[4..4 + 4*len], len as int))), data[4 + 4*len..])
+    else
+        (None, [])
+  ) else (
+    (None, [])
+  )
+}
+
+method ParseUint32Array(data:seq<byte>, index: uint64) returns (success:bool, v:V, rest_index:uint64)
+    requires (index as int) <= |data|;
+    requires |data| < 0x1_0000_0000_0000_0000;
+    ensures  (rest_index as int) <= |data|;
+    ensures  var (v', rest') := parse_Uint32Array(data[index..]);
+             var v_opt := if success then Some(v) else None();
+             && v_opt == v'
+             && data[rest_index..] == rest';
+{
+  if |data| as uint64 - index >= 4 {
+    var len32 := Unpack_LittleEndian_Uint32(data, index);
+    var len := len32 as uint64;
+    assert data[index..][..4] == data[index..index+4];
+    if len <= ((|data| as uint64) - index - 4) / Uint32Size() {
+      success := true;
+      var contents := Unpack_LittleEndian_Uint32_Seq(data, index + Uint32Size(), len);
+      v := VUint32Array(contents);
+      rest_index := index + 4 + len * Uint32Size();
+
+      assert data[index..][4..4+4*len] == data[index+4..index+4+4*len];
+    } else {
+      success := false;
+      rest_index := (|data| as uint64);
+    }
+  } else {
+    success := false;
+    rest_index := (|data| as uint64);
+  }
+}
+
 function parse_Uint64Array(data:seq<byte>) : (Option<V>, seq<byte>)
     requires |data| < 0x1_0000_0000_0000_0000;
 {
@@ -794,6 +883,7 @@ function {:opaque} parse_Val(data:seq<byte>, grammar:G) : (Option<V>, seq<byte>)
              |rest| <= |data| && (!val.None? ==> ValidVal(val.value) && ValInGrammar(val.value, grammar));
 {
     match grammar
+        case GUint32             => parse_Uint32(data)
         case GUint64             => parse_Uint64(data)
         case GArray(elt)         => parse_Array(data, elt)
         case GTuple(t)           => parse_Tuple(data, t)
@@ -802,6 +892,7 @@ function {:opaque} parse_Val(data:seq<byte>, grammar:G) : (Option<V>, seq<byte>)
           var (v, rest) := parse_Message(data);
           (if v.Some? then Some(VMessage(v.value)) else None, rest)
         )
+        case GUint32Array        => parse_Uint32Array(data)
         case GUint64Array        => parse_Uint64Array(data)
         case GKeyArray           => parse_KeyArray(data)
         case GMessageArray       => parse_MessageArray(data)
@@ -823,6 +914,7 @@ method ParseVal(data:seq<byte>, index:uint64, grammar:G) returns (success:bool, 
     reveal_parse_Val();
 
     match grammar {
+        case GUint32             => success, v, rest_index := ParseUint32(data, index);
         case GUint64             => success, v, rest_index := ParseUint64(data, index);
         case GArray(elt)         => success, v, rest_index := ParseArray(data, index, elt);
         case GTuple(t)           => success, v, rest_index := ParseTuple(data, index, t);
@@ -836,6 +928,7 @@ method ParseVal(data:seq<byte>, index:uint64, grammar:G) returns (success:bool, 
           success, v', rest_index := ParseMessage(data, index);
           v := VMessage(v'); 
         }
+        case GUint32Array          => success, v, rest_index := ParseUint32Array(data, index);
         case GUint64Array          => success, v, rest_index := ParseUint64Array(data, index);
         case GKeyArray           => success, v, rest_index := ParseKeyArray(data, index);
         case GMessageArray       => success, v, rest_index := ParseMessageArray(data, index);
@@ -964,6 +1057,60 @@ lemma lemma_parse_Val_view_Message(data:seq<byte>, v:V, grammar:G, index:int)
              ((parse_Message(data[index..bound]).0 == Some(v.m)) <==> (parse_Message(data[index..index+SizeOfV(v)]).0 == Some(v.m))));
     assert forall bound :: index+SizeOfV(v) <= bound <= |data| ==>
              parse_Message(data[index..bound]).0 == Some(v.m) ==> parse_Message(data[index..bound]).1 == data[index+SizeOfV(v)..bound];
+}
+
+lemma lemma_parse_Val_view_Uint32Array(data:seq<byte>, v:V, grammar:G, index:int)
+    requires |data| < 0x1_0000_0000_0000_0000;
+    requires ValInGrammar(v, grammar);
+    requires ValidGrammar(grammar);
+    requires grammar.GUint32Array?;
+    requires 0 <= index <= |data|;
+    requires 0 <= index + SizeOfV(v) <= |data|;
+    ensures  forall bound :: Trigger(bound) ==> (index+SizeOfV(v) <= bound <= |data| ==>
+             ((parse_Uint32Array(data[index..bound]).0 == Some(v)) <==> (parse_Uint32Array(data[index..index+SizeOfV(v)]).0 == Some(v))));
+    ensures  forall bound :: index+SizeOfV(v) <= bound <= |data| ==>
+             parse_Uint32Array(data[index..bound]).0 == Some(v) ==> parse_Uint32Array(data[index..bound]).1 == data[index+SizeOfV(v)..bound];
+{
+  forall bound | Trigger(bound) && index+SizeOfV(v) <= bound <= |data|
+  ensures (parse_Uint32Array(data[index..bound]).0 == Some(v)) ==> (parse_Uint32Array(data[index..index+SizeOfV(v)]).0 == Some(v))
+  ensures (parse_Uint32Array(data[index..index+SizeOfV(v)]).0 == Some(v)) ==> (parse_Uint32Array(data[index..bound]).0 == Some(v))
+  {
+    var len := |v.va|;
+
+    assert data[index..bound][..Uint32Size()]
+        == data[index..index + SizeOfV(v)][..Uint32Size()];
+    assert parse_Uint32(data[index..bound]).0
+        == parse_Uint32(data[index..index + SizeOfV(v)]).0;
+    assert parse_Uint32(data[index..bound]).1 == data[index..bound][4..];
+    assert parse_Uint32(data[index..index + SizeOfV(v)]).1 == data[index..index + SizeOfV(v)][4..];
+    PackedStringArray.lemma_seq_slice_slice(data, index, bound, 4, 4+4*len);
+    PackedStringArray.lemma_seq_slice_slice(data, index, index + SizeOfV(v), 4, 4+4*len);
+    assert data[index..bound][4..4+4*len] == data[index..index + SizeOfV(v)][4..4+4*len];
+
+    reveal_unpack_LittleEndian_Uint32();
+    if index + 4 <= |data| {
+      var l := unpack_LittleEndian_Uint32(data[index..index+4]);
+      if (l as int == len) {
+        /*var rest0 := data[index..bound][8..];
+        var rest1 := data[index..index + SizeOfV(v)][8..];
+        PackedStringArray.lemma_seq_slice_suffix(data, index, bound, 8);
+        PackedStringArray.lemma_seq_slice_suffix(data, index, index + SizeOfV(v), 8);
+        PackedStringArray.lemma_seq_slice_slice(data, index + 8, bound, 0, 8*len);
+        PackedStringArray.lemma_seq_slice_slice(data, index + 8, index + SizeOfV(v), 0, 8*len);
+        assert data[index..bound][Uint64Size()..][..Uint64Size() as int * len]
+            == data[index..index + SizeOfV(v)][Uint64Size()..][..Uint64Size() as int * len];
+        assert parse_Uint64Array(data[index..bound]).0.Some?;
+        assert parse_Uint64Array(data[index..index + SizeOfV(v)]).0.Some?;*/
+        assert parse_Uint32Array(data[index..bound]).0
+            == parse_Uint32Array(data[index..index + SizeOfV(v)]).0;
+      }
+    }
+  }
+
+  forall bound | index+SizeOfV(v) <= bound <= |data| && parse_Uint32Array(data[index..bound]).0 == Some(v)
+  ensures parse_Uint32Array(data[index..bound]).1 == data[index+SizeOfV(v)..bound];
+  {
+  }
 }
 
 lemma lemma_parse_Val_view_Uint64Array(data:seq<byte>, v:V, grammar:G, index:int)
@@ -1429,6 +1576,10 @@ lemma lemma_parse_Val_view(data:seq<byte>, v:V, grammar:G, index:int)
     {
         reveal_parse_Val();
         match grammar
+            case GUint32             => {
+              assume false;
+              assert (parse_Val(data[index..bound], grammar).0 == Some(v)) <==> (parse_Val(data[index..index+SizeOfV(v)], grammar).0 == Some(v));
+            }
             case GUint64             => {
               assume false;
               assert (parse_Val(data[index..bound], grammar).0 == Some(v)) <==> (parse_Val(data[index..index+SizeOfV(v)], grammar).0 == Some(v));
@@ -1443,6 +1594,7 @@ lemma lemma_parse_Val_view(data:seq<byte>, v:V, grammar:G, index:int)
                                         assert (parse_Val(data[index..bound], grammar).0 == Some(v)) <==> (parse_Val(data[index..index+SizeOfV(v)], grammar).0 == Some(v));
             case GTuple(t)           => lemma_parse_Val_view_Tuple(data, v, t, index, bound); assert (parse_Val(data[index..bound], grammar).0 == Some(v)) <==> (parse_Val(data[index..index+SizeOfV(v)], grammar).0 == Some(v));
             case GByteArray          => lemma_parse_Val_view_ByteArray(data, v, grammar, index); assert (parse_Val(data[index..bound], grammar).0 == Some(v)) <==> (parse_Val(data[index..index+SizeOfV(v)], grammar).0 == Some(v));
+            case GUint32Array          => lemma_parse_Val_view_Uint32Array(data, v, grammar, index); assert (parse_Val(data[index..bound], grammar).0 == Some(v)) <==> (parse_Val(data[index..index+SizeOfV(v)], grammar).0 == Some(v));
             case GUint64Array          => lemma_parse_Val_view_Uint64Array(data, v, grammar, index); assert (parse_Val(data[index..bound], grammar).0 == Some(v)) <==> (parse_Val(data[index..index+SizeOfV(v)], grammar).0 == Some(v));
             case GTaggedUnion(cases) => lemma_parse_Val_view_Union(data, v, grammar, index, bound); assert (parse_Val(data[index..bound], grammar).0 == Some(v)) <==> (parse_Val(data[index..index+SizeOfV(v)], grammar).0 == Some(v));
             case GPackedKV => assume false;
@@ -1568,6 +1720,7 @@ method ComputeSizeOf(val:V) returns (size:uint64)
     ensures (size as int) == SizeOfV(val);
 {
   match val {
+    case VUint32(_)     => size := 4;
     case VUint64(_)     => size := 8;
     case VArray(a)      => var v := ComputeSeqSum(a);
                            if v == 0 {
@@ -1578,6 +1731,7 @@ method ComputeSizeOf(val:V) returns (size:uint64)
     case VTuple(t)      => size := ComputeSeqSum(t);
     case VByteArray(b)  => size := 8 + (|b| as uint64);
     case VMessage(m)    => size := 4 + WeightMessageUint64(m);
+    case VUint32Array(b)  => size := 4 + 4*(|b| as uint64);
     case VUint64Array(b)  => size := 8 + 8*(|b| as uint64);
     case VKeyArray(b)  => {
       var v := ComputeWeightKeySeq(b);
@@ -1638,6 +1792,35 @@ ensures data[index..(index as int) + SizeOfV(val)][8 + i*8 .. 8 + (i+1)*8]
       == ar[a + c .. a + c + d];
   assert ar[index..(index as int) + SizeOfV(val)][8 + i*8 .. 8 + (i+1)*8]
      == ar[index as int + 8 + i*8 .. index as int + 8 + (i+1)*8];
+}
+
+method MarshallUint32(n:uint32, data:array<byte>, index:uint64)
+    requires (index as int) + (Uint32Size() as int) <= data.Length;
+    requires 0 <= (index as int) + (Uint32Size() as int) < 0x1_0000_0000_0000_0000;  // Needed to prevent overflow below
+    requires data.Length < 0x1_0000_0000_0000_0000;
+    modifies data;
+    ensures  unpack_LittleEndian_Uint32(data[index..index+(Uint32Size() as uint64)]) == n;
+    ensures  !parse_Uint32(data[index .. index+(Uint32Size() as uint64)]).0.None?;
+    ensures  !parse_Uint32(data[index .. ]).0.None?;
+    ensures  var tuple := parse_Uint32(data[index .. index+(Uint32Size() as uint64)]);
+             tuple.0.value.v == n && tuple.1 == [];
+    ensures  var tuple := parse_Uint32(data[index .. ]);
+             tuple.0.value.v == n && tuple.1 == data[index+(Uint32Size() as uint64)..];
+    ensures  data[0..index] == old(data[0..index]);
+    ensures  data[index+(Uint32Size() as uint64)..] == old(data[index+(Uint32Size() as uint64)..]);
+    ensures  forall i :: 0 <= i < index ==> data[i] == old(data[i]);
+    ensures  forall i :: (index as int) + (Uint32Size() as int) <= i < data.Length ==> data[i] == old(data[i]);
+{
+    Pack_LittleEndian_Uint32_into_Array(n, data, index);
+
+    forall i | 0 <= i < index ensures data[i] == old(data[i])
+    {
+      assert data[i] == data[..index][i] == old(data[..index])[i] == old(data[i]);
+    }
+
+    assert |data[index .. index+(Uint32Size() as uint64)]| == 4;
+
+    reveal_unpack_LittleEndian_Uint32();
 }
 
 method MarshallUint64(n:uint64, data:array<byte>, index:uint64)
@@ -2273,6 +2456,51 @@ method MarshallByteArray(val:V, ghost grammar:G, data:array<byte>, index:uint64)
     size := 8 + (|val.b| as uint64);
 }
 
+method MarshallUint32Array(val:V, ghost grammar:G, data:array<byte>, index:uint64) returns (size:uint64)
+    requires val.VUint32Array?;
+    requires ValidGrammar(grammar);
+    requires ValInGrammar(val, grammar);
+    requires ValidVal(val);
+    requires (index as int) + SizeOfV(val) <= data.Length;
+    requires 0 <= (index as int) + SizeOfV(val) < 0x1_0000_0000_0000_0000;  // Needed to prevent overflow below
+    requires data.Length < 0x1_0000_0000_0000_0000;
+    modifies data;
+    decreases grammar;
+    ensures  parse_Val(data[index..(index as int) + SizeOfV(val)], grammar).0.Some?
+    ensures  parse_Val(data[index..(index as int) + SizeOfV(val)], grammar).0.value == val;
+    ensures  forall i :: 0 <= i < index ==> data[i] == old(data[i]);
+    ensures  forall i :: (index as int) + SizeOfV(val) <= i < data.Length ==> data[i] == old(data[i]);
+    ensures  (size as int) == SizeOfV(val);
+{
+  reveal_unpack_LittleEndian_Uint32();
+  reveal_parse_Val();
+
+  ghost var data_seq0 := data[index..(index as int) + SizeOfV(val)];
+
+  MarshallUint32((|val.va| as uint32), data, index);
+
+  ghost var data_seq1 := data[index..(index as int) + SizeOfV(val)];
+  assert unpack_LittleEndian_Uint32(data_seq1[..4]) as int == |val.va|;
+
+  Pack_LittleEndian_Uint32_Seq_into_Array(val.va, data, index + 4);
+
+  ghost var data_seq2 := data[index..(index as int) + SizeOfV(val)];
+  assert unpack_LittleEndian_Uint32(data_seq2[..4]) as int == |val.va|;
+  PackedStringArray.lemma_array_slice_slice(data, index as int, (index as int) + SizeOfV(val), 4, 4 + 4*|val.va|);
+  assert unpack_LittleEndian_Uint32_Seq(
+      data_seq2[4..4 + 4*|val.va|], |val.va|) == val.va;
+
+  /*ghost var len := unpack_LittleEndian_Uint64(data_seq2[..8]);
+  assert |data_seq2| >= 4;
+  assert len <= (|data_seq2| as uint64 - 4) / 4;
+  assert parse_Uint64Array(data_seq2).0.Some?;
+  assert parse_Val(data_seq2, grammar).0.Some?;
+  assert parse_Uint64Array(data_seq2).0.value.ua == val.va;
+  assert parse_Val(data_seq2, grammar).0.value.ua == val.va;*/
+
+  size := 4 + |val.va| as uint64 * 4;
+}
+
 method MarshallUint64Array(val:V, ghost grammar:G, data:array<byte>, index:uint64) returns (size:uint64)
     requires val.VUint64Array?;
     requires ValidGrammar(grammar);
@@ -2468,6 +2696,30 @@ method MarshallMessageArray(val:V, ghost grammar:G, data:array<byte>, index:uint
   return 4 + 4*|val.ma| as uint64 + offset;
 }
 
+method MarshallVUint32(val:V, ghost grammar:G, data:array<byte>, index:uint64) returns (size:uint64)
+    requires val.VUint32?;
+    requires ValidGrammar(grammar);
+    requires ValInGrammar(val, grammar);
+    requires (index as int) + SizeOfV(val) <= data.Length;
+    requires 0 <= (index as int) + SizeOfV(val) < 0x1_0000_0000_0000_0000;  // Needed to prevent overflow below
+    requires data.Length < 0x1_0000_0000_0000_0000;
+    modifies data;
+    decreases grammar;
+    ensures  parse_Val(data[index..(index as int) + SizeOfV(val)], grammar).0.Some? &&
+             parse_Val(data[index..(index as int) + SizeOfV(val)], grammar).0.value == val;
+    ensures  forall i :: 0 <= i < index ==> data[i] == old(data[i]);
+    ensures  forall i :: (index as int) + SizeOfV(val) <= i < data.Length ==> data[i] == old(data[i]);
+    ensures  (size as int) == SizeOfV(val);
+{
+    MarshallUint32(val.v, data, index);
+    calc {
+        parse_Val(data[index..(index as int) + SizeOfV(val)], grammar);
+            { reveal_parse_Val(); }
+        parse_Uint32(data[index..(index as int) + SizeOfV(val)]);
+    }
+    return 4;
+}
+
 method MarshallVUint64(val:V, ghost grammar:G, data:array<byte>, index:uint64) returns (size:uint64)
     requires val.VUint64?;
     requires ValidGrammar(grammar);
@@ -2527,10 +2779,12 @@ method MarshallVal(val:V, ghost grammar:G, data:array<byte>, index:uint64) retur
     ensures  (size as int) == SizeOfV(val);
 {
     match val
+        case VUint32(_)    => size := MarshallVUint32(val, grammar, data, index);
         case VUint64(_)    => size := MarshallVUint64(val, grammar, data, index);
         case VArray(_)     => size := MarshallArray(val, grammar, data, index);
         case VKeyArray(_) => size := MarshallKeyArray(val, grammar, data, index);
         case VTuple(_)     => size := MarshallTuple(val, grammar, data, index);
+        case VUint32Array(_) => size := MarshallUint32Array(val, grammar, data, index);
         case VUint64Array(_) => size := MarshallUint64Array(val, grammar, data, index);
         case VByteArray(_) => size := MarshallByteArray(val, grammar, data, index);
         case VMessage(_) => size := MarshallMessage(val.m, data, index);
@@ -2563,6 +2817,13 @@ method Marshall(val:V, ghost grammar:G) returns (data:array<byte>)
 lemma lemma_SizeOfV_parse_Val_Uint64(data: seq<byte>)
 requires |data| < 0x1_0000_0000_0000_0000;
 ensures var (v, rest) := parse_Uint64(data);
+  v.Some? ==> SizeOfV(v.value) + |rest| == |data|
+{
+}
+
+lemma lemma_SizeOfV_parse_Val_Uint32(data: seq<byte>)
+requires |data| < 0x1_0000_0000_0000_0000;
+ensures var (v, rest) := parse_Uint32(data);
   v.Some? ==> SizeOfV(v.value) + |rest| == |data|
 {
 }
@@ -2661,6 +2922,13 @@ ensures var (v, rest) := parse_Message(data);
 {
 }
 
+lemma lemma_SizeOfV_parse_Val_Uint32Array(data: seq<byte>)
+requires |data| < 0x1_0000_0000_0000_0000;
+ensures var (v, rest) := parse_Uint32Array(data);
+  v.Some? ==> SizeOfV(v.value) + |rest| == |data|
+{
+}
+
 lemma lemma_SizeOfV_parse_Val_Uint64Array(data: seq<byte>)
 requires |data| < 0x1_0000_0000_0000_0000;
 ensures var (v, rest) := parse_Uint64Array(data);
@@ -2693,11 +2961,13 @@ ensures var (v, rest) := parse_Val(data, grammar);
 {
   reveal_parse_Val();
   match grammar {
+    case GUint32             => lemma_SizeOfV_parse_Val_Uint32(data);
     case GUint64             => lemma_SizeOfV_parse_Val_Uint64(data);
     case GArray(elt)         => lemma_SizeOfV_parse_Val_Array(data, elt);
     case GTuple(t)           => lemma_SizeOfV_parse_Val_Tuple(data, t);
     case GByteArray          => lemma_SizeOfV_parse_Val_ByteArray(data);
     case GMessage            => lemma_SizeOfV_parse_Val_Message(data);
+    case GUint32Array        => lemma_SizeOfV_parse_Val_Uint32Array(data);
     case GUint64Array        => lemma_SizeOfV_parse_Val_Uint64Array(data);
     case GKeyArray           => lemma_SizeOfV_parse_Val_KeyArray(data);
     case GMessageArray       => lemma_SizeOfV_parse_Val_MessageArray(data);
